Examples/Ringofsaturn_com/Analyze_Ringofsaturn_com.thy
@@ -23,12 +23,14 @@ abbreviation MatchNotPrefix :: "'a match_expr \<Rightarrow> 'a match_expr" ("\<n
   "MatchNotPrefix m \<equiv> MatchNot m"
 (*This syntax can be pretty confusing when mixing it with other theories. Do not use outside this example!*)
 
+value[code] "unfold_ruleset_INPUT saturn_fw_INPUT_default_policy (map_of_string saturn_fw)"
 lemma "unfold_ruleset_INPUT saturn_fw_INPUT_default_policy (map_of_string saturn_fw) =
- [Rule (Match (Extra ''-m state --state RELATED,ESTABLISHED'')) action.Accept,
-  Rule (Match (Extra ''-m state --state NEW'')) action.Accept,
+ [Rule (Match (CT_State {CT_Related, CT_Established})) action.Accept,
+  Rule (Match (CT_State {CT_New})) action.Accept,
   Rule (Match (Prot (Proto TCP))) action.Drop,
   Rule (Match (Prot (Proto UDP))) action.Drop,
-  Rule MatchAny action.Drop, Rule (Match (IIface (Iface ''lo''))) action.Accept,
+  Rule MatchAny action.Drop,
+  Rule (Match (IIface (Iface ''lo''))) action.Accept,
   Rule ((Match (Src (Ip4AddrNetmask (0, 0, 0, 0) 8)) MATCHAND Match (IIface (Iface ''eth0''))) MATCHAND Match (Prot (Proto TCP)))
    action.Drop,
   Rule ((Match (Src (Ip4AddrNetmask (0, 0, 0, 0) 8)) MATCHAND Match (IIface (Iface ''eth0''))) MATCHAND Match (Prot (Proto UDP)))
@@ -66,14 +68,10 @@ lemma "unfold_ruleset_INPUT saturn_fw_INPUT_default_policy (map_of_string saturn
   Rule (Match (Src (Ip4AddrNetmask (240, 0, 0, 0) 8)) MATCHAND Match (IIface (Iface ''eth0''))) action.Drop,
   Rule (Match (Src (Ip4AddrNetmask (160, 86, 0, 0) 16)) MATCHAND Match (IIface (Iface ''eth1''))) action.Accept,
   Rule (Match (IIface (Iface ''eth1''))) action.Drop,
-  Rule (Match (IIface (Iface ''eth0'')) MATCHAND Match (Prot (Proto ICMP)) MATCHAND Match (Extra ''-m icmp --icmp-type 3''))
-   action.Accept,
-  Rule (Match (IIface (Iface ''eth0'')) MATCHAND Match (Prot (Proto ICMP)) MATCHAND Match (Extra ''-m icmp --icmp-type 11''))
-   action.Accept,
-  Rule (Match (IIface (Iface ''eth0'')) MATCHAND Match (Prot (Proto ICMP)) MATCHAND Match (Extra ''-m icmp --icmp-type 0''))
-   action.Accept,
-  Rule (Match (IIface (Iface ''eth0'')) MATCHAND Match (Prot (Proto ICMP)) MATCHAND Match (Extra ''-m icmp --icmp-type 8''))
-   action.Accept,
+  Rule (Match (IIface (Iface ''eth0'')) MATCHAND Match (Prot (Proto ICMP)) MATCHAND Match (Extra ''-m icmp --icmp-type 3'')) action.Accept,
+  Rule (Match (IIface (Iface ''eth0'')) MATCHAND Match (Prot (Proto ICMP)) MATCHAND Match (Extra ''-m icmp --icmp-type 11'')) action.Accept,
+  Rule (Match (IIface (Iface ''eth0'')) MATCHAND Match (Prot (Proto ICMP)) MATCHAND Match (Extra ''-m icmp --icmp-type 0'')) action.Accept,
+  Rule (Match (IIface (Iface ''eth0'')) MATCHAND Match (Prot (Proto ICMP)) MATCHAND Match (Extra ''-m icmp --icmp-type 8'')) action.Accept,
   Rule (Match (Prot (Proto TCP)) MATCHAND Match (Dst_Ports [(0x6F, 0x6F)])) action.Drop,
   Rule (Match (IIface (Iface ''eth0'')) MATCHAND Match (Prot (Proto TCP)) MATCHAND Match (Dst_Ports [(0x71, 0x71)])) action.Drop,
   Rule (Match (IIface (Iface ''eth0'')) MATCHAND Match (Prot (Proto TCP)) MATCHAND Match (Dst_Ports [(4, 4)])) action.Accept,
@@ -90,7 +88,9 @@ lemma "unfold_ruleset_INPUT saturn_fw_INPUT_default_policy (map_of_string saturn
   Rule (Match (IIface (Iface ''eth0'')) MATCHAND Match (Prot (Proto UDP)) MATCHAND Match (Dst_Ports [(0x208, 0x208)])) action.Drop,
   Rule (Match (IIface (Iface ''eth0'')) MATCHAND Match (Prot (Proto TCP)) MATCHAND Match (Dst_Ports [(0x89, 0x8B)])) action.Drop,
   Rule (Match (IIface (Iface ''eth0'')) MATCHAND Match (Prot (Proto UDP)) MATCHAND Match (Dst_Ports [(0x89, 0x8B)])) action.Drop,
-  Rule (Match (Prot (Proto TCP))) action.Drop, Rule (Match (Prot (Proto UDP))) action.Drop, Rule MatchAny action.Drop,
+  Rule (Match (Prot (Proto TCP))) action.Drop,
+  Rule (Match (Prot (Proto UDP))) action.Drop,
+  Rule MatchAny action.Drop,
   Rule MatchAny action.Accept]" by eval
 
 lemma "good_ruleset (unfold_ruleset_INPUT saturn_fw_INPUT_default_policy (map_of_string saturn_fw))" by eval
@@ -98,53 +98,42 @@ lemma "simple_ruleset (unfold_ruleset_INPUT saturn_fw_INPUT_default_policy (map_
 
 text{*Basically, it accepts everything*}
 lemma "take 2 (unfold_ruleset_INPUT saturn_fw_INPUT_default_policy (map_of_string saturn_fw)) =
-    [Rule (Match (Extra ''-m state --state RELATED,ESTABLISHED'')) action.Accept, Rule (Match (Extra ''-m state --state NEW'')) action.Accept]" by eval
+    [Rule (Match (CT_State {CT_Related, CT_Established})) action.Accept, Rule (Match (CT_State {CT_New})) action.Accept]" by eval
 
+(*TODO: all the CT states are essentially the universe*)
 
 text{*The upper closure*}
+(*value[code] "upper_closure (unfold_ruleset_INPUT saturn_fw_INPUT_default_policy (map_of_string saturn_fw))"*)
 lemma upper: "upper_closure (unfold_ruleset_INPUT saturn_fw_INPUT_default_policy (map_of_string saturn_fw)) =
- [Rule MatchAny action.Accept,
+ [Rule (Match (CT_State {CT_Related, CT_Established})) action.Accept,
+  Rule (Match (CT_State {CT_New})) action.Accept,
   Rule (Match (Prot (Proto TCP))) action.Drop,
   Rule (Match (Prot (Proto UDP))) action.Drop,
-  Rule MatchAny action.Drop, Rule (Match (IIface (Iface ''lo''))) action.Accept,
-  Rule (Match (Src (Ip4AddrNetmask (0, 0, 0, 0) 8)) MATCHAND Match (IIface (Iface ''eth0'')) MATCHAND Match (Prot (Proto TCP)))
-   action.Drop,
-  Rule (Match (Src (Ip4AddrNetmask (0, 0, 0, 0) 8)) MATCHAND Match (IIface (Iface ''eth0'')) MATCHAND Match (Prot (Proto UDP)))
-   action.Drop,
+  Rule MatchAny action.Drop,
+  Rule (Match (IIface (Iface ''lo''))) action.Accept,
+  Rule (Match (Src (Ip4AddrNetmask (0, 0, 0, 0) 8)) MATCHAND Match (IIface (Iface ''eth0'')) MATCHAND Match (Prot (Proto TCP))) action.Drop,
+  Rule (Match (Src (Ip4AddrNetmask (0, 0, 0, 0) 8)) MATCHAND Match (IIface (Iface ''eth0'')) MATCHAND Match (Prot (Proto UDP))) action.Drop,
   Rule (Match (Src (Ip4AddrNetmask (0, 0, 0, 0) 8)) MATCHAND Match (IIface (Iface ''eth0''))) action.Drop,
-  Rule (Match (Src (Ip4AddrNetmask (10, 0, 0, 0) 8)) MATCHAND Match (IIface (Iface ''eth0'')) MATCHAND Match (Prot (Proto TCP)))
-   action.Drop,
-  Rule (Match (Src (Ip4AddrNetmask (10, 0, 0, 0) 8)) MATCHAND Match (IIface (Iface ''eth0'')) MATCHAND Match (Prot (Proto UDP)))
-   action.Drop,
+  Rule (Match (Src (Ip4AddrNetmask (10, 0, 0, 0) 8)) MATCHAND Match (IIface (Iface ''eth0'')) MATCHAND Match (Prot (Proto TCP))) action.Drop,
+  Rule (Match (Src (Ip4AddrNetmask (10, 0, 0, 0) 8)) MATCHAND Match (IIface (Iface ''eth0'')) MATCHAND Match (Prot (Proto UDP))) action.Drop,
   Rule (Match (Src (Ip4AddrNetmask (10, 0, 0, 0) 8)) MATCHAND Match (IIface (Iface ''eth0''))) action.Drop,
-  Rule (Match (Src (Ip4AddrNetmask (127, 0, 0, 0) 8)) MATCHAND Match (IIface (Iface ''eth0'')) MATCHAND Match (Prot (Proto TCP)))
-   action.Drop,
-  Rule (Match (Src (Ip4AddrNetmask (127, 0, 0, 0) 8)) MATCHAND Match (IIface (Iface ''eth0'')) MATCHAND Match (Prot (Proto UDP)))
-   action.Drop,
+  Rule (Match (Src (Ip4AddrNetmask (127, 0, 0, 0) 8)) MATCHAND Match (IIface (Iface ''eth0'')) MATCHAND Match (Prot (Proto TCP))) action.Drop,
+  Rule (Match (Src (Ip4AddrNetmask (127, 0, 0, 0) 8)) MATCHAND Match (IIface (Iface ''eth0'')) MATCHAND Match (Prot (Proto UDP))) action.Drop,
   Rule (Match (Src (Ip4AddrNetmask (127, 0, 0, 0) 8)) MATCHAND Match (IIface (Iface ''eth0''))) action.Drop,
-  Rule (Match (Src (Ip4AddrNetmask (169, 254, 0, 0) 16)) MATCHAND Match (IIface (Iface ''eth0'')) MATCHAND Match (Prot (Proto TCP)))
-   action.Drop,
-  Rule (Match (Src (Ip4AddrNetmask (169, 254, 0, 0) 16)) MATCHAND Match (IIface (Iface ''eth0'')) MATCHAND Match (Prot (Proto UDP)))
-   action.Drop,
+  Rule (Match (Src (Ip4AddrNetmask (169, 254, 0, 0) 16)) MATCHAND Match (IIface (Iface ''eth0'')) MATCHAND Match (Prot (Proto TCP))) action.Drop,
+  Rule (Match (Src (Ip4AddrNetmask (169, 254, 0, 0) 16)) MATCHAND Match (IIface (Iface ''eth0'')) MATCHAND Match (Prot (Proto UDP))) action.Drop,
   Rule (Match (Src (Ip4AddrNetmask (169, 254, 0, 0) 16)) MATCHAND Match (IIface (Iface ''eth0''))) action.Drop,
-  Rule (Match (Src (Ip4AddrNetmask (172, 16, 0, 0) 12)) MATCHAND Match (IIface (Iface ''eth0'')) MATCHAND Match (Prot (Proto TCP)))
-   action.Drop,
-  Rule (Match (Src (Ip4AddrNetmask (172, 16, 0, 0) 12)) MATCHAND Match (IIface (Iface ''eth0'')) MATCHAND Match (Prot (Proto UDP)))
-   action.Drop,
+  Rule (Match (Src (Ip4AddrNetmask (172, 16, 0, 0) 12)) MATCHAND Match (IIface (Iface ''eth0'')) MATCHAND Match (Prot (Proto TCP))) action.Drop,
+  Rule (Match (Src (Ip4AddrNetmask (172, 16, 0, 0) 12)) MATCHAND Match (IIface (Iface ''eth0'')) MATCHAND Match (Prot (Proto UDP))) action.Drop,
   Rule (Match (Src (Ip4AddrNetmask (172, 16, 0, 0) 12)) MATCHAND Match (IIface (Iface ''eth0''))) action.Drop,
-  Rule (Match (Src (Ip4AddrNetmask (224, 0, 0, 0) 3)) MATCHAND Match (IIface (Iface ''eth0'')) MATCHAND Match (Prot (Proto TCP)))
-   action.Drop,
-  Rule (Match (Src (Ip4AddrNetmask (224, 0, 0, 0) 3)) MATCHAND Match (IIface (Iface ''eth0'')) MATCHAND Match (Prot (Proto UDP)))
-   action.Drop,
+  Rule (Match (Src (Ip4AddrNetmask (224, 0, 0, 0) 3)) MATCHAND Match (IIface (Iface ''eth0'')) MATCHAND Match (Prot (Proto TCP))) action.Drop,
+  Rule (Match (Src (Ip4AddrNetmask (224, 0, 0, 0) 3)) MATCHAND Match (IIface (Iface ''eth0'')) MATCHAND Match (Prot (Proto UDP))) action.Drop,
   Rule (Match (Src (Ip4AddrNetmask (224, 0, 0, 0) 3)) MATCHAND Match (IIface (Iface ''eth0''))) action.Drop,
-  Rule (Match (Src (Ip4AddrNetmask (240, 0, 0, 0) 8)) MATCHAND Match (IIface (Iface ''eth0'')) MATCHAND Match (Prot (Proto TCP)))
-   action.Drop,
-  Rule (Match (Src (Ip4AddrNetmask (240, 0, 0, 0) 8)) MATCHAND Match (IIface (Iface ''eth0'')) MATCHAND Match (Prot (Proto UDP)))
-   action.Drop,
+  Rule (Match (Src (Ip4AddrNetmask (240, 0, 0, 0) 8)) MATCHAND Match (IIface (Iface ''eth0'')) MATCHAND Match (Prot (Proto TCP))) action.Drop,
+  Rule (Match (Src (Ip4AddrNetmask (240, 0, 0, 0) 8)) MATCHAND Match (IIface (Iface ''eth0'')) MATCHAND Match (Prot (Proto UDP))) action.Drop,
   Rule (Match (Src (Ip4AddrNetmask (240, 0, 0, 0) 8)) MATCHAND Match (IIface (Iface ''eth0''))) action.Drop,
   Rule (Match (Src (Ip4AddrNetmask (160, 86, 0, 0) 16)) MATCHAND Match (IIface (Iface ''eth1''))) action.Accept,
-  Rule (Match (IIface (Iface ''eth1''))) action.Drop,
-  Rule (Match (IIface (Iface ''eth0'')) MATCHAND Match (Prot (Proto ICMP))) action.Accept,
+  Rule (Match (IIface (Iface ''eth1''))) action.Drop, Rule (Match (IIface (Iface ''eth0'')) MATCHAND Match (Prot (Proto ICMP))) action.Accept,
   Rule (Match (Dst_Ports [(0x6F, 0x6F)]) MATCHAND Match (Prot (Proto TCP))) action.Drop,
   Rule (Match (Dst_Ports [(0x71, 0x71)]) MATCHAND Match (IIface (Iface ''eth0'')) MATCHAND Match (Prot (Proto TCP))) action.Drop,
   Rule (Match (Dst_Ports [(4, 4)]) MATCHAND Match (IIface (Iface ''eth0'')) MATCHAND Match (Prot (Proto TCP))) action.Accept,
@@ -160,7 +149,8 @@ lemma upper: "upper_closure (unfold_ruleset_INPUT saturn_fw_INPUT_default_policy
   Rule (Match (Dst_Ports [(0x1BB, 0x1BB)]) MATCHAND Match (IIface (Iface ''eth0'')) MATCHAND Match (Prot (Proto UDP))) action.Accept,
   Rule (Match (Dst_Ports [(0x208, 0x208)]) MATCHAND Match (IIface (Iface ''eth0'')) MATCHAND Match (Prot (Proto UDP))) action.Drop,
   Rule (Match (Dst_Ports [(0x89, 0x8B)]) MATCHAND Match (IIface (Iface ''eth0'')) MATCHAND Match (Prot (Proto TCP))) action.Drop,
-  Rule (Match (Dst_Ports [(0x89, 0x8B)]) MATCHAND Match (IIface (Iface ''eth0'')) MATCHAND Match (Prot (Proto UDP))) action.Drop]"
+  Rule (Match (Dst_Ports [(0x89, 0x8B)]) MATCHAND Match (IIface (Iface ''eth0'')) MATCHAND Match (Prot (Proto UDP))) action.Drop,
+  Rule MatchAny action.Accept]"
  by eval
 
 text{* The upper closure is essentially the Allow-All ruleset*}
